theories/AlmostStlc/SmallStep.v
@@ -1,14 +1,866 @@
 Require Export Syntax.
 Require Export TypedVar.
 From Equations Require Import Equations Signature.
+Require Import ExtLib.Structures.Functor.
+Require Import ExtLib.Structures.Applicative.
+Require Import ExtLib.Structures.Monad.
 
-Equations subst_term {Γ R} (t1 t2 : type) (e1 : term t2 Γ R) (e2 : term t1 Γ R) (x : var t1 Γ)
+From Coq Require Import
+     List.
+Open Scope list_scope.
+Import ListNotations.
+Import MonadNotation.
+Local Open Scope monad_scope.
+Arguments VarZ {_ _ _}.
+Arguments VarS {_ _ _ _}.
 
-Equations subst_term {Γ R} (t1 t2 : type) (e1 : term t2 (t1 :: Γ) R) (e2 : term t1 Γ R) :
-  term t2 Γ R :=
-  subst_term t1 Nat (term_const n _ R) e2 := term_const n Γ R;
-  subst_term t1 (List tl) (term_nil tl _ R) e2 := term_nil tl Γ R;
-  (* this example shows that my type is not general enough, need to be able to go under binders and need *)
-  subst_term t1 (List tl) (term_cons tl _ R eh et) e2 := term_cons tl Γ R (subst_term _ _ eh e2) (subst_term _ _ et e2)
+Definition weaken_var_r {A} : forall (l1 l2 : list A) (a : A), var a l1 -> var a (l1 ++ l2) := @append_var A.
 
+Equations weaken_var_l {A} (l1 l2 : list A) (a : A) (x : var a l2) : var a (l1 ++ l2) :=
+  weaken_var_l nil l2 a x := x;
+  weaken_var_l (b :: l1) l2 a x := VarS (weaken_var_l l1 l2 a x). 
+Transparent weaken_var_l.
+Equations swap_var {A} (l: list A) (a b c: A) (x : var a ([b] ++ [c] ++ l) ) :
+  var a ([c] ++ [b] ++ l) :=
+  swap_var l a a c VarZ :=  VarS VarZ;
+  swap_var l a b a (VarS VarZ) := VarZ;
+  swap_var l a b c (VarS (VarS y) ) := VarS (VarS y).
+
+
+Equations weaken_var_mid {A} (l1 l2 l3 : list A) (a : A) (x : var a (l1 ++ l3) ) :
+  var a (l1 ++ l2 ++ l3)  :=
+  weaken_var_mid (b :: l1) _ _ b VarZ := VarZ;
+  weaken_var_mid (b :: l1) l2 l3 a (VarS y) := VarS (weaken_var_mid _ _ _ a y);
+  weaken_var_mid nil l2 l3 a y := weaken_var_l l2 l3 a y.
+
+
+Arguments perm_trans {_ _ _ _}.
+Arguments perm_swap {_ _ _ _ _}.
+Arguments perm_refl {_ _ }.
+Arguments perm_skip {_ _ _ _}.
+Arguments perm_var {_ _ _ _}.
+Equations exchange_var_r_perm {A} (l1 l2 : list A) (a b : A) : 
+  perm ([a] ++ l1 ++ [b] ++ l2) ([b] ++ l1 ++ [a] ++ l2) :=
+  exchange_var_r_perm [] l2 a b := perm_swap perm_refl;
+  exchange_var_r_perm (c :: l1) l2 a b :=
+    let IHl2 := exchange_var_r_perm l1 l2 a b in
+    perm_trans (perm_swap perm_refl) (perm_trans (perm_skip IHl2) (perm_swap perm_refl)).
+
+Equations exchange_var_perm {A} (G1 G2 G3 : list A) (u1 u2 : A) :
+  perm (G1 ++ [u1] ++ G2 ++ [u2] ++ G3) (G1 ++ [u2] ++ G2 ++ [u1] ++ G3 ) :=
+  exchange_var_perm [] G2 G3 u1 u2 := exchange_var_r_perm G2 G3 u1 u2;
+  exchange_var_perm (c :: G1) G2 G3 u1 u2 :=
+    perm_skip (exchange_var_perm G1 G2 G3 u1 u2).
+
+Definition exchange_var {A} (G1 G2 G3 : list A) (u1 u2 t : A) 
+           (x : var t (G1 ++ [u1] ++ G2 ++ [u2] ++ G3)) : 
+  var t (G1 ++ [u2] ++ G2 ++ [u1] ++ G3 ) :=
+  perm_var x (exchange_var_perm G1 G2 G3 u1 u2).
+
+Arguments term_const (_) {_ _}.
+Arguments term_cons {_ _ _}.
+Arguments term_nil {_ _ _}.
+Arguments term_var {_ _ _}.
+Arguments term_succ {_ _}.
+Arguments term_match_nat {_ _ _}.
+Arguments term_match_list {_ _ _ _}.
+Arguments term_pair {_ _ _ _}.
+Arguments term_split {_ _ _ _ _}.
+Arguments term_app {_ _ _ _}.
+Arguments term_abs {_ _ _ _ _}.
+Arguments term_perm {_ _ _ _}.
+Arguments term_call {_ _ _ _ _}.
+Arguments term_mfix {_ _} (_) {_}.
+Arguments mfix_bodies_nil {_ _}.
+Arguments mfix_bodies_cons {_ _ _ _ _}.
+
+
+Scheme term_mind := Induction for term Sort Type
+  with mfix_bodies_mind := Induction for mfix_bodies Sort Type.
+
+Combined Scheme term_mfix_bodies_mutind from term_mind, mfix_bodies_mind.
+
+
+Equations var_map_skip {A} (l1 l2 : list A) (b : A) (f : forall c, var c l1 -> var c l2) a
+          (x : var a (b :: l1)) : var a (b :: l2) :=
+  var_map_skip l1 l2 _ _ f VarZ := VarZ;
+  var_map_skip l1 l2 _ _ f (VarS y) := VarS (f _ y).
+
+Arguments var_map_skip {_ _ _ _}.
+
+Equations term_map {t : type} {G1 G2 : ctx} {MR : mfix_ctx} (e : term t G1 MR) 
+          (f : forall t', var t' G1 -> var t' G2) : term t G2 MR :=
+  term_map (term_const n) f := term_const n;
+  term_map term_nil f := term_nil;
+  term_map (term_cons eh et) f := term_cons (term_map eh f) (term_map et f);
+  term_map (term_var x) f := term_var (f _ x);
+  term_map (term_succ en) f := term_succ (term_map en f);
+  term_map (term_match_nat en eZ eS) f :=
+    term_match_nat (term_map en f) (term_map eZ f) 
+                   (term_map eS (var_map_skip f));
+  term_map (term_match_list el enil econs) f :=
+    term_match_list (term_map  el f) (term_map enil f)
+                    (term_map econs (var_map_skip (var_map_skip f)));
+  term_map (term_pair e1 e2) f:=
+    term_pair (term_map e1 f) (term_map e2 f);
+  term_map (term_split ep e) f :=
+    term_split (term_map ep f) (term_map e (var_map_skip (var_map_skip f)) );
+  term_map (term_app e1 e2) f :=
+    term_app (term_map e1 f) (term_map e2 f);
+  term_map (term_abs ebody) f :=
+    term_abs (term_map ebody (var_map_skip f));
+  term_map (term_perm Hperm e) f := term_perm Hperm (term_map e f);
+  term_map (term_lift _ _ _ _ e) f := term_lift _ _ _ _ (term_map e f);
+  term_map (term_call xR x arg) f := term_call xR x (term_map arg f);
+  term_map (term_mfix _ x bodies e) f :=
+    term_mfix _ x (bodies_map bodies f) (term_map e f);
+  where bodies_map {G1 G2 : ctx} {MR : mfix_ctx} {R : call_frame} (bodies : mfix_bodies G1 MR R)
+                 (f : forall t', var t' G1 -> var t' G2) : mfix_bodies G2 MR R :=
+    bodies_map mfix_bodies_nil f := mfix_bodies_nil;
+    bodies_map (mfix_bodies_cons body bodies) f :=
+      mfix_bodies_cons (term_map body (var_map_skip f)) (bodies_map bodies f).
+Transparent term_map.
+
+
+Definition exchange_term MR G1 G2 G3 (u1 u2 t:type)
+      (e : term t (G1 ++ [u1] ++ G2 ++ [u2] ++ G3) MR) : 
+      term t (G1 ++ [u2] ++ G2 ++ [u1] ++ G3) MR :=
+  term_map e (fun t' x => perm_var x (exchange_var_perm G1 G2 G3 u1 u2)).
+Definition weaken_l_term MR G1 G2 t (e : term t G2 MR ) : term t (G1 ++ G2) MR
+  := term_map e (fun t' e' => weaken_var_l _ _ t' e').
+Definition weaken_l_term_single MR t1 G2 t (e : term t G2 MR ) : term t (t1 :: G2) MR :=
+  weaken_l_term MR [t1] G2 t e.
+
+Definition weaken_l_bodies {R MR G1 G2} (bodies : mfix_bodies G2 MR R) : mfix_bodies (G1 ++ G2) MR R :=
+  bodies_map bodies (fun t' e' => weaken_var_l _ _ t' e').
+
+Definition weaken_l_bodies_single {R MR G t} (bodies : mfix_bodies G MR R) : mfix_bodies (t :: G) MR R:=
+  @weaken_l_bodies _ _ [t] G bodies.
+
+Definition weaken_r_term MR G1 G2 t (e : term t G1 MR ) : term t (G1 ++ G2) MR
+  := term_map e (fun t' e' => weaken_var_r _ _ t' e').
+Definition weaken_mid_term MR G1 G2 G3 t (e : term t (G1 ++ G3) MR) : term t (G1 ++ G2 ++ G3) MR
+  := term_map e (fun t' e' => weaken_var_mid _ _ _ t' e').
+
+Fixpoint term_of_value {t Γ MR} (v : value t) : term t Γ MR :=
+  match v with
+  | val_const n => term_const n
+  | val_nil => term_nil
+  | val_cons hv tv => term_cons (term_of_value hv) (term_of_value tv)
+  | val_pair v1 v2 => term_pair (term_of_value v1) (term_of_value v2)
+  | val_abs e => weaken_r_term _ _ _ _ (term_abs e) 
+  end. 
+
+Equations subst_var {MR t u} (G1 G2 : list type) (e : value t) (x : var u (G1 ++ [t] ++ G2 )) :
+                term u (G1 ++ G2) MR := 
+    subst_var (t1 :: G1) _ e VarZ := term_var VarZ;
+    subst_var (t1 :: G1) G2 e (VarS y) := weaken_l_term_single _ _ _ _ (subst_var G1 G2 e y) ;
+    subst_var nil G2 e VarZ := weaken_r_term MR [] G2 t (term_of_value e) ;
+    subst_var nil (t1 :: G2) e (VarS y) := term_var y.
+
+(* tomorrow draft up a value and change the subst stuff *)
+Equations subst_term {t u} G1 G2 MR (e1 : term u (G1 ++ [t] ++ G2) MR ) (v : value t) :
+  term u (G1 ++ G2) MR :=
+  subst_term _ _ _ (term_const n) _ := term_const n;
+  subst_term _ _ _ term_nil _ := term_nil;
+  subst_term _ _ _ (term_cons eh et) e2 := 
+    term_cons (subst_term _ _ _ eh e2) (subst_term _ _ _ et e2);
+  subst_term _ _ _ (term_var x) e2 := subst_var _ _ e2 x;
+  subst_term _ _ _ (term_succ en) e2 := term_succ (subst_term _ _ _ en e2);
+  subst_term _ _ _ (term_match_nat en eZ eS) e2 :=
+    term_match_nat (subst_term _ _ _ en e2) (subst_term _ _ _ eZ e2)
+                   (subst_term (Nat :: G1) _ _ eS e2);
+  subst_term _ _ _ (term_match_list el enil econs) e2 :=
+    term_match_list (subst_term _ _ _ el e2) (subst_term _ _ _ enil e2)
+                    (subst_term (_ :: List _ :: G1) _ _ econs e2 );
+  subst_term _ _ _ (term_pair el er) e2 :=
+    term_pair (subst_term _ _ _ el e2) (subst_term _ _ _ er e2);
+  subst_term _ _ _ (term_split ep e) e2 :=
+    term_split (subst_term _ _ _ ep e2) (subst_term (_ :: _ :: G1) _ _ e e2 );
+  subst_term _ _ _ (term_app ef ex) e2 :=
+    term_app (subst_term _ _ _ ef e2) (subst_term _ _ _ ex e2);
+  subst_term _ _ _ (term_abs ebody) e2 :=
+    term_abs (subst_term (_ :: G1) _ _ ebody e2 );
+  subst_term _ _ _ (term_perm Hp e) e2 :=
+    term_perm Hp (subst_term _ _ _ e e2);
+  subst_term _ _ _ (term_lift _ _ _ _ e) e2 :=
+    term_lift _ _ _ _ (subst_term _ _ _ e e2);
+  subst_term _ _ _ (term_call xR xt e) e2 :=
+    term_call xR xt (subst_term _ _ _ e e2);
+  subst_term _ _ _ (term_mfix R x bodies e) e2:=
+    term_mfix R x (subst_bodies _ _ _ bodies e2) (subst_term _ _ _ e e2);
+  where subst_bodies {t R} G1 G2 MR (bodies : mfix_bodies (G1 ++ [t] ++ G2) MR R) (v : value t) : 
+    mfix_bodies (G1 ++ G2) MR R 
+    :=
+    subst_bodies _ _ _ mfix_bodies_nil _ := mfix_bodies_nil;
+    subst_bodies _ _ _ (mfix_bodies_cons ebody bodies') e2 :=
+      mfix_bodies_cons (subst_term (_ :: _) _ _ ebody e2) (subst_bodies _ _ _ bodies' e2).
+Arguments subst_term {_ _ _ _ _}.
+Definition subst_cons {t u Γ MR} (e1 : term u (t :: Γ) MR) (v : value t) :=
+  @subst_term t u [] Γ MR e1 v.
+
+
+
+Derive NoConfusion for type.
+Section redex.
+Context (err : forall A, A).
+
+Arguments err {A}.
+Notation "a && b" := (existT _ a b).
+(* maybe should enforce this is Γ = [] *)
+(* add bredexs for perm, lift, and mfix applied to values*)
+Inductive bredex : type -> ctx -> mfix_ctx -> Type :=
+  | bredex_succ {Γ MR} (vn : value Nat) : bredex Nat Γ MR
+  | bredex_match_nat {t Γ MR} (vn : value Nat) (eZ : term t Γ MR) (eS : term t (Nat :: Γ) MR) : 
+    bredex t Γ MR
+  | bredex_match_list {t1 t2 Γ MR} (vl : value (List t1)) (enil : term t2 Γ MR) 
+                     (econs : term t2 (t1 :: (List t1) :: Γ ) MR) : 
+    bredex t2 Γ MR
+  | bredex_split {t1 t2 t3 Γ MR} (vp : value (Pair t1 t2)) (e : term t3 (t1 :: t2 :: Γ) MR ) : 
+    bredex t3 Γ MR
+  | bredex_app {t1 t2 Γ MR} (vf : value (Arrow t1 MR t2) ) (vx : value t1) :
+    bredex t2 Γ MR
+  | bredex_perm {t Γ MR1 MR2} (Hperm : perm MR1 MR2) (v : value t) : 
+    bredex t Γ MR2
+  | bredex_lift {t Γ MR1 MR2} (v : value t) : 
+    bredex t Γ (MR1 ++ MR2)
+  | bredex_mfix {t Γ R MR} (x : var R MR) (bodies : mfix_bodies Γ MR R) (v : value t) :
+    bredex t Γ (TypedVar.remove R MR x)
+  .
+
+Equations step_bredex {t Γ MR} (r : bredex t Γ MR) : term t Γ MR :=
+  step_bredex (bredex_succ (val_const n) ) := term_const (1 + n);
+  step_bredex (bredex_match_nat (val_const n) eZ eS ) :=
+    match n with
+    | 0 => eZ
+    | S m => subst_cons eS (val_const m)
+    end;
+  step_bredex (bredex_match_list (val_nil) enil _ ) := enil;
+  step_bredex (bredex_match_list (val_cons vh vt) _ econs) :=
+    subst_cons (subst_cons econs vh) vt;
+  step_bredex (bredex_split (val_pair v1 v2) e) :=
+    subst_cons (subst_cons e v1) v2;
+  step_bredex (bredex_app (val_abs ebody) varg ) :=
+    weaken_r_term _ _ _ _ (subst_cons ebody varg);
+  step_bredex (bredex_perm _ v) := term_of_value v;
+  step_bredex (bredex_lift v) := term_of_value v;
+  step_bredex (bredex_mfix _ _ v) := term_of_value v.
+
+
+Inductive eval_context : type -> forall Γ :ctx, mfix_ctx -> forall t MR, (bredex t Γ MR + call MR t) -> bool -> Type := 
+  | ev_hole t Γ MR (r : (bredex t Γ MR + call MR t) ) : eval_context t Γ MR t MR r true
+  | ev_cons_l b t1 t2 Γ MR1 MR2 (r : (bredex t2 Γ MR2 + call MR2 t2)  ) 
+           (Eh : eval_context t1 Γ MR1 _ _ r b) (et : term (List t1) Γ MR1) : 
+    eval_context (List t1) Γ MR1 _ _ r b
+  | ev_cons_r b t1 t2 Γ MR1 MR2 (r : (bredex t2 Γ MR2 + call MR2 t2)  ) 
+           (vh : value t1) (Et : eval_context (List t1) Γ MR1 _ _ r b) : 
+    eval_context (List t1) Γ MR1 _ _ r b
+  | ev_succ b Γ MR1 t2 MR2 (r : (bredex t2 Γ MR2 + call MR2 t2)  )  
+         (E : eval_context Nat Γ MR1 _ _ r b) : 
+    eval_context Nat Γ MR1 _ _ r b
+  | ev_match_nat b t1 Γ MR1 t2 MR2 (r : (bredex t2 Γ MR2 + call MR2 t2)  )
+              (En : eval_context Nat Γ MR1 _ _ r b)
+              (eZ : term t1 Γ MR1)
+              (eS : term t1 (Nat :: Γ) MR1) :
+    eval_context t1 Γ MR1 _ _ r b
+  | ev_match_list b t1 t2 Γ1 MR1 t3 MR2 (r : (bredex t3 Γ1 MR2 + call MR2 t3)  )
+                  (El : eval_context (List t1) Γ1 MR1 _ _ r b)
+                  (enil : term t2 Γ1 MR1)
+                  (econs : term t2 (t1 :: (List t1) :: Γ1) MR1) : 
+    eval_context t2 Γ1 MR1 _ _ r b
+  | ev_pair_l b t1 t2 Γ1 MR1 t3 MR2 (r : (bredex t3 Γ1 MR2 + call MR2 t3)  )
+            (E1 : eval_context t1 Γ1 MR1 _ _ r b)
+            (e2 : term t2 Γ1 MR1) :
+    eval_context (Pair t1 t2) Γ1 MR1 _ _ r b
+  | ev_pair_r b t1 t2 Γ1 MR1 t3 MR2  (r : (bredex t3 Γ1 MR2 + call MR2 t3)  )
+            (v1 : value t1)
+            (E2 : eval_context t2 Γ1 MR1 _ _ r b) :
+    eval_context (Pair t1 t2) Γ1 MR1 _ _ r b
+  | ev_split b t1 t2 t3 Γ1 MR1 t4 MR2 (r : (bredex t4 Γ1 MR2 + call MR2 t4)  )
+             (Ep : eval_context (Pair t1 t2) Γ1 MR1 _ _ r b)
+             (es : term t3 (t1 :: t2 :: Γ1) MR1 ) : 
+    eval_context t3 Γ1 MR1 _ _ r b
+  | ev_app_l b t1 t2 Γ1 MR1 t3 MR2 (r : (bredex t3 Γ1 MR2 + call MR2 t3))
+             (Ef : eval_context (Arrow t1 MR1 t2) Γ1 MR1 _ _ r b)
+             (e : term t1 Γ1 MR1) : 
+    eval_context t2 Γ1 MR1 _ _ r b
+  | ev_app_r b t1 t2 Γ1 MR1 t3 MR2 (r : (bredex t3 Γ1 MR2 + call MR2 t3))
+             (vf : value (Arrow t1 MR1 t2))
+             (E : eval_context t1 Γ1 MR1 _ _ r b) : 
+    eval_context t2 Γ1 MR1 _ _ r b
+  | ev_perm b t1 Γ1 MR1 MR2 t2 MR3  (r : (bredex t2 Γ1 MR3 + call MR3 t2))
+            (Hperm : perm MR1 MR2)
+            (E : eval_context t1 Γ1 MR1 _ _ r b) : 
+    eval_context t1 Γ1 MR2 _ _ r false
+  | ev_lift b t1 Γ1 MR1 MR2 t2 MR3 (r : (bredex t2 Γ1 MR3 + call MR3 t2))
+            (E : eval_context t1 Γ1 MR2 _ _ r b) : 
+    eval_context t1 Γ1 (MR1 ++ MR2) _ _ r false
+  | ev_call b t1 t2 Γ1 MR1 R t3 MR2 (r : (bredex t3 Γ1 MR2 + call MR2 t3))
+            (xR : var R MR1) (x : var (t1,t2) R)
+            (E : eval_context t1 Γ1 MR1 _ _ r b) : 
+    eval_context t2 Γ1 MR1 _ _ r b
+  | ev_mfix b t1 Γ1 MR1 R1 t2 MR2 (r : (bredex t2 Γ1 MR2 + call MR2 t2)) 
+            (x : var R1 MR1) (bodies : mfix_bodies Γ1 MR1 R1)
+            (E : eval_context t1 Γ1 MR1 _ _ r b) :
+    eval_context t1 Γ1 (TypedVar.remove R1 MR1 x) _ _ r false
 .
+Arguments ev_hole {_ _ _ _}.
+Arguments ev_cons_l {b t1 t2 Γ MR1 MR2 r}.
+Arguments ev_cons_r {b t1 t2 Γ MR1 MR2 r}.
+Arguments ev_succ {b Γ MR1 t2 MR2 r}.
+Arguments ev_match_nat {b t1 Γ MR1 t2 MR2 r}.
+Arguments ev_match_list {b t1 t2 Γ1 MR1 t3  MR2 r}.
+Arguments ev_pair_l {b t1 t2 Γ1 MR1 t3 MR2 r}.
+Arguments ev_pair_r {b t1 t2 Γ1 MR1 t3 MR2 r}.
+Arguments ev_split {b t1 t2 t3 Γ1 MR1 t4 MR2 r}.
+Arguments ev_app_l {b t1 t2 Γ1 MR1 t3 MR2 r}.
+Arguments ev_app_r {b t1 t2 Γ1 MR1 t3 MR2 r}.
+Arguments ev_perm (b) {t1 Γ1 MR1 MR2 t2 MR3 r}.
+Arguments ev_lift (b) {t1 Γ1 MR1 MR2 t2 MR3 r}.
+Arguments ev_call {b t1 t2 Γ1 MR1 R t3 MR2 r}.
+Arguments ev_mfix (b) {t1 Γ1 MR1 R1 t2 MR2 r}.
+Arguments eval_context (_ _ _) {_ _}.
+Equations subst_eval_context {b t1 t2 Γ1 MR1 MR2} (r : (bredex t2 Γ1 MR2 + call MR2 t2)) 
+           (E : eval_context t1 Γ1 MR1 r b) (e : term t2 Γ1 MR2) : term t1 Γ1 MR1 :=
+  subst_eval_context r ev_hole e := e;
+  subst_eval_context r (ev_cons_l Eh et) e := term_cons (subst_eval_context r Eh e) et;
+  subst_eval_context r (ev_cons_r vh Et) e := term_cons (term_of_value vh) (subst_eval_context r Et e);
+  subst_eval_context r (ev_succ E) e := term_succ (subst_eval_context r E e);
+  subst_eval_context r (ev_match_nat En eZ eS) e := 
+    term_match_nat (subst_eval_context r En e) eZ eS;
+  subst_eval_context r (ev_match_list El enil econs) e := 
+    term_match_list (subst_eval_context r El e) enil econs;
+  subst_eval_context r (ev_pair_l E1 e2) e :=
+    term_pair (subst_eval_context r E1 e) e2;
+  subst_eval_context r (ev_pair_r v1 E2) e :=
+    term_pair (term_of_value v1) (subst_eval_context r E2 e);
+  subst_eval_context r (ev_split Ep es) e :=
+    term_split (subst_eval_context r Ep e) es;
+  subst_eval_context r (ev_app_l E1 e2) e :=
+    term_app (subst_eval_context r E1 e) e2;
+  subst_eval_context r (ev_app_r v1 E2) e :=
+    term_app (term_of_value v1) (subst_eval_context r E2 e);
+  subst_eval_context r (ev_perm _ Hperm E) e :=
+    term_perm Hperm (subst_eval_context r E e);
+  subst_eval_context r (ev_lift _ E) e :=
+    term_lift _ _ _ _(subst_eval_context r E e);
+  subst_eval_context r (ev_call xR x E) e :=
+    term_call xR x (subst_eval_context r E e);
+  subst_eval_context r (ev_mfix _ x bodies E) e :=
+    term_mfix _ x bodies (subst_eval_context r E e). 
+
+(* change this to be particular to call *)
+Equations normalize_eval_context {t1 t2 Γ1 MR1 MR2} (c : call MR2 t2) 
+           (E : eval_context t1 Γ1 MR1 (inr c) true) : 
+  {c : call MR1 t2 & eval_context t1 Γ1 MR1 (inr c) true} :=
+
+  normalize_eval_context c ev_hole := c && ev_hole;
+  normalize_eval_context c (ev_cons_l Eh et) := 
+    let '(c' && Eh') := normalize_eval_context c Eh in
+    c' && (ev_cons_l Eh' et);
+  normalize_eval_context c (ev_cons_r vh Et) :=
+    let '(c' && Et') := normalize_eval_context c Et in
+    c' && ev_cons_r vh Et';
+  normalize_eval_context c (ev_succ En) :=
+    let '(c' && En') := normalize_eval_context c En in
+    c' && ev_succ En';
+  normalize_eval_context c (ev_match_nat En eZ eS) :=
+    let '(c' && En') := normalize_eval_context c En in
+    c' && ev_match_nat En' eZ eS;
+  normalize_eval_context c (ev_match_list El enil econs) :=
+    let '(c' && El') := normalize_eval_context c El in
+    c' && ev_match_list El' enil econs;
+  normalize_eval_context c (ev_pair_l E1 e2) :=
+    let '(c' && E1') := normalize_eval_context c E1 in
+    c' && ev_pair_l E1' e2;
+  normalize_eval_context c (ev_pair_r v1 E2) :=
+    let '(c' && E2') := normalize_eval_context c E2 in
+    c' && ev_pair_r v1 E2';
+  normalize_eval_context c (ev_split E es) :=
+    let '(c' && E') := normalize_eval_context c E in
+    c' && ev_split E' es;
+  normalize_eval_context c (ev_app_l E1 e2) :=
+    let '(c' && E1') := normalize_eval_context c E1 in
+    c' && ev_app_l E1' e2;
+  normalize_eval_context c (ev_app_r v1 E2) :=
+    let '(c' && E2') := normalize_eval_context c E2 in
+    c' && ev_app_r v1 E2';
+  normalize_eval_context c (ev_call xR x E) :=
+    let '(c' && E') := normalize_eval_context c E in
+    c' && ev_call xR x E'.
+(*
+Equations lift_term_map {Γ MR1 MR2 t1} (f : forall t, term t Γ MR1 -> term t Γ MR2) (t : type) 
+          (e : term t (t1 :: Γ) MR1) : term t (t1 :: Γ) MR2 :=
+  lift_term_map f _ (term_const n) := term_const n;
+  lift_term_map f _ term_nil := term_nil;
+  lift_term_map f _ (term_cons eh et) := term_cons (lift_term_map f _ eh) (lift_term_map f _ et);
+  lift_term_map f _ (term_var VarZ) := term_var VarZ;
+  lift_term_map f _ (term_var (VarS x)) := weaken_l_term_single _ _ _ _ (f _ (term_var x));
+  lift_term_map f _ (term_succ en) := term_succ (lift_term_map f _ en);
+  lift_term_map f _ (term_match_nat en eZ eS) :=
+    term_match_nat (lift_term_map f _ en) (lift_term_map f _ eZ)
+                   (lift_term_map (lift_term_map f) _ eS);
+  lift_term_map f _ (term_match_list el enil econs) :=
+    term_match_list (lift_term_map f _ el) (lift_term_map f _ enil)
+                    (lift_term_map (lift_term_map (lift_term_map f) ) _ econs);
+  lift_term_map f _ (term_pair e1 e2) :=
+    term_pair (lift_term_map f _ e1) (lift_term_map f _ e2);
+  lift_term_map f _ (term_split ep e) :=
+    term_split (lift_term_map f _ ep) (lift_term_map (lift_term_map (lift_term_map f) ) _ e );
+  lift_term_map f _ (term_app e1 e2) :=
+    term_app (lift_term_map f _ e1) (lift_term_map f _ e2);
+  lift_term_map f _ (term_abs ebody) := term_abs ebody;
+  lift_term_map f _ _ := err.
+*)
+
+Definition term_map_perm {Γ MR1 MR2} (Hperm : perm MR1 MR2) : forall t, term t Γ MR1 -> term t Γ MR2 :=
+  fun t e => term_perm Hperm e.
+Definition term_map_lift {Γ MR1 MR2} : forall t, term t Γ MR2 -> term t Γ (MR1 ++ MR2) :=
+  fun t e => term_lift _ _ _ _ e.
+
+Definition term_map_mfix {Γ R MR} (x : var R MR) (bodies : mfix_bodies Γ MR R) : 
+  forall t, term t Γ MR -> term t Γ (TypedVar.remove R MR x) :=
+  fun t e => term_mfix R x bodies e.
+(* try to work out your new push idea I think it is by far the best idea you currently have,
+   it would give you a way to simply push mfix, perm, and lift 
+   I also think I need to keep track of depth, if the application in two deep (i.e. two args)
+   then I need to change the effect signature of the two lambda, one nested in the other (assuming no call events)
+*)
+(* weird error message here, pay close attention when get to it *)
+Equations push_eval_context {t1 t2 Γ1 MR1 MR2} (r : bredex t2 Γ1 MR1 + call MR1 t2)
+           (E : eval_context t1 Γ1 MR1 r true) 
+           (f : forall t Γ, term t (Γ ++ Γ1) MR1 -> term t (Γ ++ Γ1) MR2) (* a bit suspicious of Γ here*)
+           (fvar : forall R, var R MR1 -> var R MR2) (* mfix will work differently, maybe there just needs to be a another function for that*)
+           (e : term t2 Γ1 MR2) : term t1 Γ1 MR2 :=
+  push_eval_context _ ev_hole f fvar e := e;
+  push_eval_context _ (ev_cons_l Eh et) f fvar e :=
+    term_cons (push_eval_context _ Eh f fvar e) (f _ [] et); (* need to change the mfix context of et*)
+  push_eval_context _ (ev_cons_r v Et) f fvar e :=
+    term_cons (term_of_value v) (push_eval_context _ Et f fvar e);
+  push_eval_context _ (ev_succ E) f fvar e :=
+    term_succ (push_eval_context _ E f fvar e);
+  push_eval_context _ (ev_match_nat En eZ eS) f fvar e :=
+    term_match_nat (push_eval_context _ En f fvar e) (f _ [] eZ) (f _ [Nat] eS); 
+  push_eval_context _ (ev_match_list El enil econs) f fvar e :=
+    term_match_list (push_eval_context _ El f fvar e) (f _ [] enil) (f _ [_;_] econs);
+  push_eval_context _ (ev_pair_l E1 e2) f fvar e :=
+    term_pair (push_eval_context _ E1 f fvar e) (f _ [] e2);
+  push_eval_context _ (ev_pair_r v1 E2) f fvar e :=
+    term_pair (term_of_value v1) (push_eval_context _ E2 f fvar e);
+  push_eval_context _ (ev_split Ep es) f fvar e :=
+    term_split (push_eval_context _ Ep f fvar e) (f _ [_ ; _] es );
+  (* the problem with app is showing up in a different location now, uggh*)
+  push_eval_context _ (ev_app_r (val_abs ebody) E2) f fvar e :=
+    term_app (term_abs (f _ [t3] (weaken_r_term _ _ _ _ ebody) )) (push_eval_context _ E2 f fvar e);
+  push_eval_context _ (ev_call xR x E) f fvar e := 
+    term_call (fvar _ xR) x (push_eval_context _ E f fvar e) ;
+  push_eval_context _ (ev_app_l E1 e2) f fvar e := err.
+    (* term_app (push_eval_context _ E1 f fvar e) (f _ [] e2) *);
+  
+
+Instance option_monad : Monad option :=
+  {|
+    ret := fun _ x => Some x;
+    bind := fun _ _ m k =>
+              match m with
+              | None => None
+              | Some x => k x end;
+  |}.
+
+(*
+Definition step_eval_context_l {t1 t2 Γ1 Γ2 MR1 MR2} b (br : bredex t2 Γ2 MR2) 
+           (E : eval_context t1 Γ1 MR1 (inl br) b ): option (term t1 Γ1 MR1) :=
+  Some (subst_eval_context (inl br) E (step_bredex br)).
+
+Equations step_eval_context_r {t1 t2 Γ1 Γ2 MR1 MR2} b (c : call MR2 t2)
+           (E : @eval_context t1 Γ1 MR1 t2 Γ2 MR2 (inr c) b) : option (term t1 Γ1 MR1) :=
+  step_eval_context_r _ (ev_mfix false x bodies E) := e <- step
+  step_eval_context_r _ c E := err.
+
+Equations step_eval_context {t1 t2 Γ1 Γ2 MR1 MR2} b (r : (bredex t2 Γ2 MR2 + call MR2 t2)) 
+           (E : eval_context t1 Γ1 MR1 r b) : option (term t1 Γ1 MR1) :=
+  step_eval_context b (inl br) E := step_eval_context_l b br E;
+  step_eval_context b (inr c) E := step_eval_context_r b c E.
+*)
+
+(**)
+(* need to rely on var_eq_neq *)
+(*
+Equations var_eq_
+*)
+(* Equations is very slow on creating the equations for this function,
+   if developing with it, use the #[derive(equations=no)] directive
+   to save time
+*)
+Equations step_eval_context {t1 t2 Γ1 MR1 MR2} b (r : (bredex t2 Γ1 MR2 + call MR2 t2)) 
+           (E : eval_context t1 Γ1 MR1 r b) : option (term t1 Γ1 MR1) :=
+  step_eval_context _ (inl br) E := ret (subst_eval_context (inl br) E (step_bredex br));
+
+  step_eval_context _ (inr c) (ev_mfix true xR bodies E) := 
+      let '( (callv yR x v) && E' ) := normalize_eval_context c E in
+      ret 
+      match (var_eq_neq _ _ _ xR yR) with
+      | inl Heq => 
+          let fx := nth_body bodies (var_eq_elim xR yR Heq x) in
+          let e := subst_cons fx v in
+          term_mfix R1 xR bodies (subst_eval_context (inr (callv yR x v) ) E' e)
+      | inr Hneq =>
+          let yR' := remove_var _ _ _ xR yR Hneq in
+          push_eval_context (inr (callv yR x v)) E' (fun t e => term_mfix R1 xR bodies e)
+                            (term_call yR' x (term_of_value v)) end;
+
+  step_eval_context _ (inr c) (ev_mfix false x bodies E) := 
+        e <- step_eval_context false (inr c) E;;
+        ret (term_mfix _ x bodies e);
+
+  step_eval_context _ (inr c) (ev_perm true Hperm E) :=
+          let '((callv yR x v) && E' ) := normalize_eval_context c E in
+          ret (
+          push_eval_context (inr (callv yR x v)) E' (fun t e => term_perm Hperm e)
+                            (term_call (perm_var yR Hperm) x (term_of_value v)));
+
+  step_eval_context _ (inr c) (ev_perm false Hperm E) :=
+            e <- step_eval_context false (inr c) E;;
+            ret (term_perm Hperm e);
+
+  step_eval_context _ (inr c) (ev_lift true E) :=
+          let '((callv yR x v) && E' ) := normalize_eval_context c E in
+          ret (
+              push_eval_context _ E' (fun t e => term_lift _ _ _ _ e)
+                                (term_call (weaken_var_l _ _ _ yR) x (term_of_value v) ));
+
+  step_eval_context _ (inr c) (ev_lift false E) :=
+                e <- step_eval_context false (inr c) E;;
+                ret (term_lift _ _ _ _ e);
+
+  step_eval_context _ (inr c) _ := None.
+
+    (* here I should use push, relying on Hneq to transform yR into a remove R1 MR1 xR variable*)
+    
+(*
+tomorrow, first use what we currently have to write a step function,
+see if any weird issues come up
+start with mfix, lift, and perm because those are the werid ones
+
+eval_context -> option term,
+
+then write that lifting function, and finish up the push_eval_context
+
+from there start a new file for relating 
+*)
+
+End redex.
+
+Definition halted t MR : Type := (value t + call MR t).
+
+
+(* unfortunately, I don't know if this will play nicely with the handler idea 
+   on second thought, it might, but I think it will require more cases
+*)
+Inductive term_obs : type -> ctx -> mfix_ctx -> Type := 
+(* need to rethink this part for the recursion problem, the *)
+| obs_consl t Γ MR (eh : term_obs t Γ MR) (et : term (List t) Γ MR) : term_obs (List t) Γ MR
+| obs_consr t Γ MR (vh : halted t MR) (et : term_obs (List t) Γ MR) : term_obs (List t) Γ MR
+| obs_cons_calll t Γ MR (c : call MR t) (ht : halted (List t) MR)   : term_obs (List t) Γ MR
+| obs_cons_callr t Γ MR (v1 : value t) (ct : call MR (List t)) : term_obs (List t) Γ MR
+| obs_succe Γ MR (e : term Nat Γ MR) : term_obs Nat Γ MR
+| obs_succh Γ MR (hn : halted Nat MR) : term_obs Nat Γ MR
+| obs_match_nate t Γ MR (en : term Nat Γ MR) (eZ : term t Γ MR) (eS : term t (Nat :: Γ) MR ) :
+  term_obs t Γ MR
+| obs_match_nath t Γ MR (hn : halted Nat MR) (eZ : term t Γ MR) (eS : term t (Nat :: Γ) MR) :
+  term_obs t Γ MR
+| obs_match_liste t1 t2 Γ MR (el : term (List t1) Γ MR) (enil : term t2 Γ MR) 
+                  (econs : term t2 (t1 :: List t1 :: Γ) MR ) :
+  term_obs t2 Γ MR
+| obs_match_listh t1 t2 Γ MR (hl : halted (List t1) MR) (enil : term t2 Γ MR) 
+                  (econs : term t2 (t1 :: List t1 :: Γ) MR ) :
+  term_obs t2 Γ MR
+| obs_pairl t1 t2 Γ MR (e1 : term t1 Γ MR) (e2 : term t2 Γ MR) :
+  term_obs (Pair t1 t2) Γ MR
+| obs_pairr t1 t2 Γ MR (h1 : halted t1 MR) (e2 : term t2 Γ MR) : 
+  term_obs (Pair t1 t2) Γ MR
+| obs_pair_callr t1 t2 Γ MR (v1 : value t1) (c2 : call MR t2) : 
+  term_obs (Pair t1 t2) Γ MR
+| obs_splite t1 t2 t3 Γ MR (ep : term (Pair t1 t2) Γ MR) (esp : term t3 (t1 :: t2 :: Γ) MR) : 
+             term_obs t3 Γ MR
+| obs_splith t1 t2 t3 Γ MR (hp : halted (Pair t1 t2) MR) (esp : term t3 (t1 :: t2 :: Γ) MR) : 
+             term_obs t3 Γ MR
+| obs_appl t1 t2 Γ MR (ef : term (Arrow t1 MR t2) Γ MR) (ex : term t1 Γ MR) : 
+  term_obs t2 Γ MR
+| obs_appr t1 t2 Γ MR (hf : halted (Arrow t1 MR t2) MR) (ex : term t1 Γ MR) : 
+  term_obs t2 Γ MR
+(*
+| obs_app_callr t1 t2 Γ MR (vf : value (Arrow t1 MR t2) ) (cx : call MR t1) :
+  term_obs t2 Γ MR
+*)
+| obs_calle t1 t2 Γ R MR (xR : var R MR) (x : var (t1,t2) R) (arge : term t1 Γ MR) :
+  term_obs t2 Γ MR
+| obs_perme t Γ MR1 MR2 (Hperm : perm MR1 MR2)  (e : term t Γ MR1) : 
+  term_obs t Γ MR2
+| obs_permh t Γ MR1 MR2 (Hperm : perm MR1 MR2)  (he : halted t MR1) : 
+  term_obs t Γ MR2
+| obs_lifte t Γ MR1 MR2 (e : term t Γ MR2) :
+  term_obs t Γ (MR1 ++ MR2)
+| obs_lifth t Γ MR1 MR2 (eh : halted t MR2) : 
+  term_obs t Γ (MR1 ++ MR2)
+| obs_mfixe t Γ R MR x (bodies : mfix_bodies Γ MR R)  (e : term t Γ MR) : 
+  term_obs t Γ (TypedVar.remove R MR x)
+| obs_mfixh t Γ R MR x (bodies : mfix_bodies Γ MR R)  (eh : halted t MR) : 
+  term_obs t Γ (TypedVar.remove R MR x)
+.
+Arguments obs_consl {t Γ MR}.
+Arguments obs_consr {t Γ MR}.
+Arguments obs_cons_calll {t Γ MR}.
+Arguments obs_cons_callr {t Γ MR}.
+Arguments obs_succe {Γ MR}.
+Arguments obs_succh {Γ MR}.
+Arguments obs_match_nate {t Γ MR}.
+Arguments obs_calle {t1 t2 Γ R MR}.
+Arguments obs_match_nath {t Γ MR}.
+Arguments obs_match_liste {t1 t2 Γ MR}.
+Arguments obs_match_listh {t1 t2 Γ MR}.
+Arguments obs_pairl {t1 t2 Γ MR}.
+Arguments obs_pairr {t1 t2 Γ MR}.
+Arguments obs_pair_callr {t1 t2 Γ MR}.
+Arguments obs_splite {t1 t2 t3 Γ MR}.
+Arguments obs_splith {t1 t2 t3 Γ MR}.
+Arguments obs_appl {t1 t2 Γ MR}.
+Arguments obs_appr {t1 t2 Γ MR}.
+Arguments obs_perme {t Γ MR1 MR2}.
+Arguments obs_permh {t Γ MR1 MR2}.
+Arguments obs_lifte {t Γ MR1 MR2}.
+Arguments obs_lifth {t Γ MR1 MR2}.
+Arguments obs_mfixe {t Γ R MR}.
+Arguments obs_mfixh {t Γ R MR}.
+(* Arguments obs_app_callr {t1 t2 Γ MR}. *)
+(* what should it give for (call 0, call 1), 
+   right now, I think that should count as a term_obs,
+   and should step to call 0
+
+   just to be clear match e ...
+
+   if halted e
+   then if value e then do substitution
+        else if halted e then e
+   else match (step e) ...
+
+maybe call needs to be changed 
+maybe it needs to be all of the possible ways a term can get stuck because of a call
+
+
+*)
+
+Section observe.
+
+Context (err : forall A, A).
+Arguments err {A}.
+(* actually realizing this does not quite work as I have written it, 
+   call (call 0) what should its type be, suggests the call needs some more constructors
+
+   as it is currently written, call MR t objects must have an argument evaluated to a 
+   value, this is problematic because the argument might itself evaluate to a call
+   how should we design this type then
+
+   what if 
+   call MR t :=
+   call_intro t1 t2 (cont : value t2 -> call MR t)
+
+   something like that where a call object requires some kind of continuation
+   this doesn't seem well founded, needs a base case of some kind or maybe some rethinking
+   
+
+*)
+
+(*
+Arguments term _ (_ _)%list_scope
+Arguments term_const n%nat_scope {Γ MR}%list_scope
+Arguments term_nil {t} {Γ MR}%list_scope
+Arguments term_cons {t} {Γ MR}%list_scope head tail
+Arguments term_var {t} {Γ MR}%list_scope x
+Arguments term_succ {Γ MR}%list_scope en
+Arguments term_match_nat {t} {Γ MR}%list_scope en eZ eS
+Arguments term_match_list {t1 t2} {Γ MR}%list_scope el enil econs
+Arguments term_pair {t1 t2} {Γ MR}%list_scope e1 e2
+Arguments term_split {t1 t2 t3} {Γ MR}%list_scope ep e
+Arguments term_app {t1 t2} {Γ MR}%list_scope e1 e2
+Arguments term_abs {t1 t2} {Γ MR MR'}%list_scope e
+Arguments term_perm {t} {Γ MR1 MR2}%list_scope Hperm e
+Arguments term_lift t (Γ MR1 MR2)%list_scope e
+Arguments term_call {t1 t2} {Γ MR R}%list_scope xR x arg
+Arguments term_mfix {t} {Γ}%list_scope R%list_scope {MR}%list_scope x bodies e
+Arguments mfix_bodies (_ _ _)%list_scope
+Arguments mfix_bodies_nil {Γ MR}%list_scope
+Arguments mfix_bodies_cons {Γ MR}%list_scope {t1 t2} {R'}%list_scope body bodies
+*)
+Notation to x := (inl x).
+Notation val x := (inr (inl x)).
+Notation ca x := (inr (inr x)).
+(* processes a closed term into a form where we can, without recursion, easily 
+   identify what reduction step should be taken *)
+Equations observe {t MR} (e : term t [] MR) : term_obs t [] MR + (value t + call MR t) :=
+  (* simple values *)
+  observe (term_const n) := val (val_const n);
+  observe term_nil := val val_nil;
+  observe (term_abs ebody) := val (val_abs ebody);
+  (* call *)
+  observe (term_call xR x arg) :=
+    match observe arg with
+    | to eobs => to ((obs_calle xR x arg) )
+    | val v => ca (callv xR x v)
+    | ca c => ca (calls xR x c) end;
+  (* composition expressions *)
+  observe (term_cons eh et) :=
+    match observe eh, observe et with 
+    | to eobs, _ => to (obs_consl eobs et)
+    | ca c, inr h => to (obs_cons_calll c h)
+    | val v1, val v2 => val (val_cons v1 v2)
+    | val v1, ca c => to (obs_cons_callr v1 c)
+    | inr h, to eobs => to (obs_consr h eobs) 
+    end;
+    (*
+    match observe eh with
+    | to eobs => to (obs_consl eobs et)
+    | ca c => to (obs_consr (inr c) et)
+    | val v1  => 
+        match observe et with
+        | to eobs => to (obs_consr (inl v1) eobs )
+        | ca c => to (obs_cons_callr v1 c)
+        | val v2 => val (val_cons v1 v2) end
+    end; *)
+  observe (term_succ en) :=
+    match observe en with
+    | to eobs => to (obs_succe en)
+    | inr hn => to (obs_succh hn) end;
+  observe (term_match_nat en eZ eS) :=
+    match observe en with
+    | to _ => to (obs_match_nate en eZ eS)
+    | inr hn => to (obs_match_nath hn eZ eS) end;
+  observe (term_match_list el enil econs) :=
+    match observe el with
+    | to _ => to (obs_match_liste el enil econs)
+    | inr hl => to (obs_match_listh hl enil econs ) end;
+  observe (term_pair e1 e2) :=
+    match observe e1 with
+    | to eobs => to (obs_pairl e1 e2)
+    | ca c => to (obs_pairr (inr c) e2)
+    | val v1 =>
+        match observe e2 with
+        | to _ => to (obs_pairr (inl v1) e2)
+        | ca c => to (obs_pair_callr v1 c)
+        | val v2 => val (val_pair v1 v2) end
+    end;
+  observe (term_split ep es) :=
+    match observe ep with
+    | to _ => to (obs_splite ep es)
+    | inr hs => to (obs_splith hs es) end;
+  observe (term_app ef ex) :=
+    match observe ef with
+    | to _ => to (obs_appl ef ex)
+    | inr hf => to (obs_appr hf ex) end;
+  observe (term_perm Hperm e) :=
+    match observe e with
+    | to _ => to (obs_perme Hperm e)
+    | inr hr => to (obs_permh Hperm hr) end;
+  observe (term_lift _ _ _ _ e) :=
+    match observe e with
+    | to _ => to (obs_lifte e)
+    | inr h => to (obs_lifth h) end;
+  observe (term_mfix _ x bodies e) :=
+    match observe e with
+    | to _ => to (obs_mfixe x bodies e)
+    | inr h => to (obs_mfixh x bodies h) end.
+
+Definition handlers : Type := unit.
+
+Equations step {t MR} (hs : handlers) (e : term t [] MR) : term t [] MR + value t :=
+  step hs (term_const n) := inr (val_const n);
+
+
+  (* call *)
+  step hs (term_call )
+  step hs _ := err.
+
+
+(*
+Arguments term_obs _ (_ _)%list_scope
+Arguments obs_consl {t} {Γ MR}%list_scope eh et
+Arguments obs_consr {t} {Γ MR}%list_scope vh et
+Arguments obs_cons_callr {t} {Γ MR}%list_scope v1 ct
+Arguments obs_succe {Γ MR}%list_scope e
+Arguments obs_succh {Γ MR}%list_scope hn
+Arguments obs_match_nate {t} {Γ MR}%list_scope en eZ eS
+Arguments obs_match_nath {t} {Γ MR}%list_scope hn eZ eS
+Arguments obs_match_liste {t1 t2} {Γ MR}%list_scope el enil econs
+Arguments obs_match_listh {t1 t2} {Γ MR}%list_scope hl enil econs
+Arguments obs_pairl {t1 t2} {Γ MR}%list_scope e1 e2
+Arguments obs_pairr {t1 t2} {Γ MR}%list_scope h1 e2
+Arguments obs_pair_callr {t1 t2} {Γ MR}%list_scope v1 c2
+Arguments obs_splite {t1 t2 t3} {Γ MR}%list_scope ep esp
+Arguments obs_splith {t1 t2 t3} {Γ MR}%list_scope hp esp
+Arguments obs_appl {t1 t2} {Γ MR}%list_scope ef ex
+Arguments obs_appr {t1 t2} {Γ MR}%list_scope hf ex
+Arguments obs_calle {t1 t2} {Γ R MR}%list_scope xR x arge
+Arguments obs_perme {t} {Γ MR1 MR2}%list_scope Hperm e
+Arguments obs_permh {t} {Γ MR1 MR2}%list_scope Hperm he
+Arguments obs_lifte {t} {Γ MR1 MR2}%list_scope e
+Arguments obs_lifth {t} {Γ MR1 MR2}%list_scope eh
+Arguments obs_mfixe {t} {Γ R MR}%list_scope x bodies e
+Arguments obs_mfixh {t} {Γ R MR}%list_scope x bodies eh
+
+*)
+Definition term_of {t MR} (x : term t [] MR + (value t + call MR t)) :=
+  match x with
+  | inl e => e
+  | inr (inl v) => term_of_value v
+  | inr (inr c) => term_of_call c end.
+
+Definition step_with {t MR} (f : term_obs t [] MR -> term t [] MR + (value t + call MR t)) 
+           (e : term t [] MR) : term t [] MR + (value t + call MR t) :=
+  match observe e with
+  | inl eobs => f eobs
+  | inr (inl v) => inr (inl v)
+  | inr (inr c) => inr (inr c) end.
+(* there is an issue here that I am calling step_obs on observe eh and not on eh itself,
+   will need to think carefully about how to circumvent that, hopefully it does not
+   ruin this way of doing things
+
+   maybe the solution is obs_consl has an observed expr in the left arg
+*)
+
+(* maybe consider big step semantics and make it relational? *)
+(* might be a good idea to create a monad for *)
+Equations step_obs {t MR} (eo : term_obs t [] MR) : term t [] MR + (value t + call MR t) 
+  by struct eo :=
+  step_obs (obs_consl eh et) :=
+    let eh' := term_of (step_obs eh) in 
+    inl (term_cons eh' et);
+  step_obs (obs_consr h et) :=
+    let et' := term_of (step_obs et) in
+    inl (term_cons (term_of (inr h)) et');
+  step_obs (obs_cons_calll c _) :=
+    (* uncovered another mismatch can't always step to a call because the type won't match,
+       need to find the best way to represent this 
+
+
+       remember that is it very important that mfix and lift and perm go down
+       first, I guess perm and lift before mfix
+
+       I am having a hard time seeing how installing these handlers should actually work
+
+       maybe think about it from a evaluation context perspective
+     *)
+    ca c;
+  
+  step_obs _ := err.
+Admitted.
+
+
+Definition step {t MR} (e : term t [] MR) : term t [] MR + (value t + call MR t) :=
+  match observe e with
+  | inl eobs => step_obs eobs
+  | inr (inl v) => inr (inl v)
+  | inr (inr c) => inr (inr c) end.
+
+End observe.
+
+
