theories/AlmostStlc/Syntax.v
@@ -39,3 +39,51 @@ with mfix_bodies : ctx -> mfix_ctx -> call_frame -> Type :=
   | mfix_bodies_cons Γ MR t1 t2 R' (body : term t2 (t1 :: Γ) MR) (bodies : mfix_bodies Γ MR R') :
     mfix_bodies Γ MR ((t1,t2) :: R')
 .
+
+
+(* values should include const, nil cons (var?) succ of a value pair split abs (perm?) (lift?)
+
+most important thing is that they do not include calls which enables them to be substituted safely
+*)
+Inductive value : type -> Type := 
+  | val_const (n : nat) : value Nat
+  | val_nil t : value (List t)
+  | val_cons t (hv : value t) (tv : value (List t)) : value (List t)
+  | val_pair t1 t2 (v1 : value t1) (v2 : value t2) : value (Pair t1 t2)
+  | val_abs t1 t2 MR (e : term t2 (t1 :: nil) MR) : value (Arrow t1 MR t2)
+.
+Arguments val_nil {t}.
+Arguments val_cons {t}.
+Arguments val_pair {t1 t2}.
+Arguments val_abs {t1 t2 MR}.
+
+
+
+  (* this represents something with that has a call at the top,
+     and therefore
+
+
+     mfix fs in (call e) -> mfix fs in call (mfix fs in e)
+     mfix fs in (call v) -> mfix fs in (f v)
+
+     mfix fs in v -> v
+
+   *)
+(* not super convinced that this is the right way to do it *)
+Inductive call MR (t2 : type) : Type := 
+  | callv t1 R  (xR : var R MR)  (x : var (t1,t2) R) (v : value t1)
+  (* | calls t1 R  (xR : var R MR)  (x : var (t1,t2) R) (c : call MR t1) *).
+Arguments callv {_ _ _ _}.
+(* Arguments calls {_ _ _ _}. *)
+(*
+Equations term_of_call {MR t} (c : call MR t) : term t nil MR :=
+  term_of_call (@callv MR t2 t1 R xR x v) := term_call _ _ nil MR R xR x (term_of_value v);
+  term_of_call (@calls MR t2 t1 R xR x c) := term_call _ _ nil MR R xR x (term_of_call c).
+Transparent term_of_call.
+*)
+(* essential when reducing denote_bodies *)
+Equations nth_body {Γ MR R t1 t2} (bodies : mfix_bodies Γ MR R) (x : var (t1, t2) R) : term t2 (t1 :: Γ) MR :=
+  nth_body (mfix_bodies_cons _ _ _ _ _ e _) (VarZ _) := e;
+  nth_body (mfix_bodies_cons _ _ _ _ _ _ bodies) (VarS _ _ x) := nth_body bodies x.
+(* reasoning about *)
+
