theories/AlmostStlc/DenotationFacts.v
@@ -1,0 +1,278 @@
+Require Export MrecMonad.
+Require Export HeterogeneousRelations.
+Require Export EnTreeDefinition.
+Require Export Syntax.
+Require Export Denotation.
+From Coq Require Import Lists.List Logic.JMeq Eqdep CRelationClasses.
+
+Require Export MapEFacts.
+Require Export InterpMTreeFacts.
+Require Export Eq.Eqit.
+From Equations Require Import Equations Signature.
+Require Import Coq.Program.Equality.
+Import Monads.
+Import MonadNotation.
+Local Open Scope monad_scope.
+
+
+Lemma remove_denote_encodes R MR (x : var R MR)
+      (d : denote_mrec_ctx
+         (remove (denote_call_frame R && encodes_call_frame R) (denote_mfix_ctx MR) (denote_var x))) :
+  encodes d = encodes (projT1 (remove_denote x d) ).
+Proof.
+  dependent induction x.
+  - Transparent remove_denote. simpl in *. Opaque remove_denote. auto.
+  - Transparent remove_denote. simpl in *. Opaque remove_denote. 
+    destruct d. auto. 
+    specialize (IHx d). destruct (remove_denote x d). auto.
+Qed.
+
+Lemma remove_denote_cont R MR (x : var R MR)
+      (d : denote_mrec_ctx
+         (remove (denote_call_frame R && encodes_call_frame R) (denote_mfix_ctx MR) (denote_var x))) : 
+  projT2 (remove_denote x d) ~= @id (encodes d).
+Proof.
+  dependent induction x.
+  - Transparent remove_denote. simpl in *. Opaque remove_denote. auto.
+  - Transparent remove_denote. simpl in *. Opaque remove_denote.
+    destruct d. auto. specialize (IHx d). destruct (remove_denote x d).
+    auto.
+Qed.
+
+Lemma remove_denote'_encodes R MR (x : var R MR)
+                                 (d : denote_mrec_ctx (denote_mfix_ctx (remove R MR x))) : 
+  encodes d = encodes (projT1 (remove_denote' x d)).
+Proof.
+  dependent induction x.
+  - Transparent remove_denote'. simpl in *. Opaque remove_denote'. auto.
+  - Transparent remove_denote'. simpl in *. Opaque remove_denote'. 
+    destruct d. auto. 
+    specialize (IHx d). destruct (remove_denote' x d). auto.
+Qed.
+
+Lemma remove_denote'_cont R MR (x : var R MR)
+                                 (d : denote_mrec_ctx (denote_mfix_ctx (remove R MR x))) : 
+  projT2 (remove_denote' x d) ~= @id (encodes d).
+Proof.
+  dependent induction x.
+  - Transparent remove_denote'. simpl in *. Opaque remove_denote'. auto.
+  - Transparent remove_denote'. simpl in *. Opaque remove_denote'. 
+    destruct d. auto. 
+    specialize (IHx d). destruct (remove_denote' x d). auto.
+Qed.
+
+Lemma call_mrec_call_frame_encodes t1 t2 R  (x : var (t1,t2) R) (c : denote_type t1) : 
+  encodes (projT1 (call_mrec_call_frame x c)) = denote_type t2.
+Proof.
+  dependent induction x.
+  - simp call_mrec_call_frame. auto.
+  - destruct b. simp call_mrec_call_frame.
+    specialize (IHx t1 t2 x eq_refl JMeq_refl c).
+    destruct (call_mrec_call_frame x c) eqn : Heq. auto.
+Qed.
+
+Lemma call_mrec_call_frame_cont t1 t2 R  (x : var (t1,t2) R) (c : denote_type t1) : 
+  projT2 (call_mrec_call_frame x c) ~= @id (denote_type t2).
+Proof.
+  dependent induction x.
+  - simp call_mrec_call_frame. auto.
+  - destruct b. simp call_mrec_call_frame.
+    specialize (IHx t1 t2 x eq_refl JMeq_refl c).
+    destruct (call_mrec_call_frame x c) eqn : Heq.
+    auto.
+Qed.
+(*do I need a bring_to_front proof? *)
+
+Lemma call_mrec_encodes t1 t2 R MR (xt : var (t1,t2) R) (xR : var R MR) (c : denote_type t1) :
+  encodes (projT1 (call_mrec xt xR c)) = denote_type t2.
+Proof.
+  dependent induction xR.
+  - simp call_mrec.
+    specialize (call_mrec_call_frame_encodes t1 t2 _ xt c) as H.
+    destruct (call_mrec_call_frame xt c). auto.
+  - simp call_mrec. specialize (IHxR xt c).
+    destruct (call_mrec xt xR c). auto.
+Qed.
+
+Lemma call_mrec_cont t1 t2 R MR (xt : var (t1,t2) R) (xR : var R MR) (c : denote_type t1) :
+  projT2 (call_mrec xt xR c) ~= @id (denote_type t2).
+Proof.
+  dependent induction xR.
+  - simp call_mrec.
+    specialize (call_mrec_call_frame_cont t1 t2 _ xt c) as H.
+    destruct (call_mrec_call_frame xt c). auto.
+  - specialize (IHxR xt c). simp call_mrec.
+    destruct (call_mrec xt xR). auto.
+Qed.
+
+Lemma bring_to_front_call_mrec t1 t2 (R : call_frame) (MR : mfix_ctx)
+      (v : denote_type t1) (xt : var (t1,t2) R) (xR : var R MR) : 
+  projT1 (bring_to_front _ (denote_var xR) (projT1 (call_mrec xt xR v))) =
+                 inl (projT1 (call_mrec_call_frame xt v)).
+Proof.
+  dependent induction xR.
+  - simp call_mrec. simp denote_var.
+    destruct (call_mrec_call_frame xt v).
+    simpl projT1. simp bring_to_front. cbn. simp bring_to_front. auto. 
+  - specialize (IHxR xt). simp denote_var. 
+    simp call_mrec. destruct (call_mrec xt xR v). simpl projT1.
+    cbn in IHxR. cbn. simp bring_to_front.
+    destruct (bring_to_front (denote_mfix_ctx l) (denote_var xR) x). cbn in IHxR. subst.
+    auto.
+Qed.
+
+Lemma bring_to_front_call_mrec_neq t1 t2 (R1 R2  : call_frame) (MR : mfix_ctx)
+      (v : denote_type t1) (xt : var (t1,t2) R1) (xR : var R1 MR) (yR : var R2 MR) (Hneq : var_neq xR yR) : 
+  projT1 (bring_to_front _ (denote_var yR) (projT1 (call_mrec xt xR v))) =
+    inr (projT1 (remove_denote' yR (projT1 (call_mrec xt (remove_var R2 R1 MR yR xR (var_neq_sym xR yR Hneq)) v)))).
+Proof.
+  dependent induction Hneq.
+  - simp var_neq_sym.
+    Transparent remove_var. simpl remove_var. Opaque remove_var.
+    Transparent call_mrec. simpl call_mrec. Opaque call_mrec.
+    destruct (call_mrec_call_frame xt v) eqn : Hc.
+    simpl projT1. Transparent remove_denote'. simpl remove_denote'. Opaque remove_denote'.
+    Transparent denote_var. simpl denote_var. Opaque denote_var.
+    simp bring_to_front. cbn. simp bring_to_front. auto. 
+  - simp var_neq_sym.
+    Transparent remove_var. simpl remove_var. Opaque remove_var.
+    Transparent call_mrec. simpl call_mrec. Opaque call_mrec.
+    Transparent denote_var. simpl denote_var. Opaque denote_var.
+    destruct (call_mrec xt x v) eqn : Hc. simpl projT1.
+    setoid_rewrite bring_to_front_equation_3. cbn.
+    Transparent remove_denote'. simpl remove_denote'. Opaque remove_denote'.
+    cbn. match goal with |- _ =  inr (projT1 ?cm) => destruct cm eqn : Hc' end.
+    cbn. Transparent TypedVar.remove. cbn in Hc'. Opaque TypedVar.remove.
+    rewrite Hc in Hc'. injection Hc'. intros. subst. auto.
+  - specialize (IHHneq xt). simp var_neq_sym. simp remove_var.
+    simp call_mrec. Transparent denote_var. simpl denote_var. Opaque denote_var.
+    Transparent remove_var. simpl remove_var. Opaque remove_var.
+    Transparent remove_denote'. simpl remove_denote'. Opaque remove_denote'.
+    destruct (call_mrec xt x v) eqn : Hc. simpl projT1 in *.
+    Transparent call_mrec. simpl call_mrec. Opaque call_mrec.
+    destruct (call_mrec xt (remove_var b a l y x (var_neq_sym x y Hneq)) v) eqn : Hc'.
+    simpl projT1 in *.
+    destruct (remove_denote' y x1) eqn : Hc''. simpl projT1 in *.
+    simp bring_to_front. cbn. simp bring_to_front.
+    destruct (bring_to_front (denote_mfix_ctx l) (denote_var y) x0). cbn in IHHneq. subst.
+    auto.
+Qed.
+
+(* write lemmas for the continuations, saying the types work out and the functions 
+   are identity 
+   have a var_neq 
+*)
+
+(* need lemmas about denote_bodies and call_mrec_call_frame
+   might need some more reasoning about mfix bodies and var
+
+ *)
+
+#[global] Instance valid_remove_denote R MR (xR : var R MR) : valid_handler (remove_denote xR).
+Proof.
+  intros d1. dependent induction xR.
+  - Transparent remove_denote. cbn. Opaque remove_denote. auto.
+  - Transparent remove_denote. cbn. Opaque remove_denote. auto.
+    destruct d1.
+    + cbn. auto.
+    + specialize (IHxR d). destruct (remove_denote xR d). auto.
+Qed.
+
+(* need to fmap the typecast *)
+Lemma denote_mfix t1 t2 (R : call_frame) (MR : mfix_ctx) (xt : var (t1,t2) R) (xR : var R MR) (v : denote_type t1) f :
+  let '(d && g) := call_mrec_call_frame xt v in
+  mapE (remove_denote xR) (interp_mtree _ _ _ (denote_var xR) f (call_term xt xR v)) ≈
+       mapE (remove_denote xR) (interp_mtree _ _ _ (denote_var xR) f (Functor.fmap g (f d))).
+Proof.
+  destruct (call_mrec_call_frame xt v) eqn : Hcall1. unfold call_term.
+  destruct (call_mrec xt xR v) eqn : Hcall2. setoid_rewrite interp_mtree_bind at 1.
+  setoid_rewrite interp_mtree_ret. specialize (bring_to_front_call_mrec _ _ R MR v xt xR) as Hbtf. 
+  rewrite Hcall2 in Hbtf. rewrite Hcall1 in Hbtf. cbn in Hbtf.
+  setoid_rewrite interp_mtree_vis. destruct (bring_to_front (denote_mfix_ctx MR) (denote_var xR) x0) eqn : Hb.
+  cbn in Hbtf. subst. rewrite tau_eutt. setoid_rewrite interp_mtree_bind at 1. setoid_rewrite bind_bind.
+  setoid_rewrite interp_mtree_bind. setoid_rewrite interp_mtree_ret.
+  eapply mapE_proper_inst. apply valid_handler_self_eq. apply valid_remove_denote.
+  setoid_rewrite bind_ret_l. eapply eqit_bind. reflexivity.
+  intros. subst. apply eqit_Ret. cbn in e. 
+  eapply JMeq_comp'; eauto.
+  - specialize (call_mrec_encodes t1 t2 R MR xt xR v) as H.
+    rewrite Hcall2 in H. auto.
+  - specialize (call_mrec_call_frame_encodes t1 t2 R xt v) as H.
+    rewrite Hcall1 in H. cbn in H. auto.
+  - specialize (call_mrec_cont t1 t2 R MR xt xR v) as H.
+    rewrite Hcall2 in H. auto.
+  - specialize (call_mrec_call_frame_cont t1 t2 R xt v) as H. 
+    rewrite Hcall1 in H. auto.
+  - specialize (bring_to_front_cont (denote_var xR) x0 ) as H. 
+    rewrite Hb in H. auto.
+Qed.
+(* need to figure this out *)
+
+Lemma remove_denote_remove_denote'_projT1:
+  forall (R2 : call_frame) (MR : mfix_ctx) (yR : var R2 MR)
+    (x0 : denote_mrec_ctx (denote_mfix_ctx (remove R2 MR yR))),
+    projT1 (remove_denote yR (projT1 (remove_denote' yR x0))) = x0.
+Proof.
+  intros R2 MR yR x0.
+  dependent induction yR.
+  - Transparent remove_denote'. cbn. Transparent remove_denote. cbn.
+    Opaque remove_denote'. Opaque remove_denote. auto.
+  - Transparent remove_denote'. cbn. Transparent remove_denote. cbn.
+    Opaque remove_denote'. Opaque remove_denote.
+    destruct x0.
+    + cbn. auto.
+    + cbn. specialize (IHyR d).
+      destruct (remove_denote' yR d). simpl.
+      simpl in IHyR. destruct (remove_denote yR x). cbn in *. subst. auto.
+Qed.
+
+Lemma JMeq_comp'':
+  forall (A B C D : Type)
+    (d : C -> D)
+    (d0 : A -> D)
+    (e : B -> C)
+    (e0 : A -> B) (a : A),
+    A = B -> B = C -> C = D -> d ~= @id D -> d0 ~= @id D -> e ~= @id C -> e0 ~= @id B -> d (e (e0 a)) = d0 a.
+Proof.
+  intros. subst. auto.
+Qed.
+
+Lemma denote_mfix_neq t1 t2 (R1 R2 : call_frame) (MR : mfix_ctx) (xt : var (t1,t2) R1) (xR : var R1 MR)
+      (yR : var R2 MR) (Hneq : var_neq xR yR) (v : denote_type t1) f :
+  mapE (remove_denote yR) (interp_mtree _ _ _ (denote_var yR) f (call_term xt xR v)) ≈
+       call_term xt (remove_var R2 R1 MR yR xR (var_neq_sym xR yR Hneq)) v.
+Proof.
+  unfold call_term.
+  specialize (bring_to_front_call_mrec_neq t1 t2 R1 R2 MR v xt xR yR Hneq) as H. 
+  destruct (call_mrec xt xR v) eqn : Hcall1.
+  destruct (call_mrec xt (remove_var R2 R1 MR yR xR (var_neq_sym xR yR Hneq)) v) eqn :  Hcall2.
+  setoid_rewrite interp_mtree_bind. setoid_rewrite interp_mtree_vis.
+  setoid_rewrite interp_mtree_ret.
+  cbn in H. destruct (bring_to_front (denote_mfix_ctx MR) (denote_var yR) x )
+                     eqn : Heq.
+  cbn in H. subst. 
+  rewrite mapE_bind; try apply valid_remove_denote.
+  rewrite mapE_vis. 
+  specialize (remove_denote_remove_denote'_projT1 R2 MR yR x0) as Hx0.
+  destruct (remove_denote yR (projT1 (remove_denote' yR x0))) eqn : Heq'. simpl in Hx0. subst.
+  setoid_rewrite bind_vis. apply eqit_Vis. intros.
+  setoid_rewrite bind_ret_l. rewrite mapE_ret. apply eqit_Ret.
+  specialize (call_mrec_cont t1 t2 R1 MR xt xR v) as Hcont1.
+  rewrite Hcall1 in Hcont1. cbn in Hcont1.
+  specialize (call_mrec_cont t1 t2 _ _ xt 
+                             (remove_var R2 R1 MR yR xR (var_neq_sym xR yR Hneq)) v ) as Hcont2.
+  rewrite Hcall2 in Hcont2. cbn in Hcont2.
+  cbn in Heq. specialize (bring_to_front_cont (denote_var yR) x) as Hcont3.
+  rewrite Heq in Hcont3. cbn in Hcont3. 
+  specialize (remove_denote_cont _ _ yR (projT1 (remove_denote' yR x0))) as Hcont4.
+  rewrite Heq' in Hcont4. cbn in Hcont4.
+  eapply JMeq_comp''; eauto.
+  - apply remove_denote'_encodes.
+  - setoid_rewrite <- remove_denote'_encodes.
+    specialize (call_mrec_encodes t1 t2 _ _ xt xR v) as Henc.
+    rewrite Hcall1 in Henc. cbn in Henc. rewrite Henc.
+    specialize (call_mrec_encodes t1 t2 _ _ xt (remove_var R2 R1 MR yR xR (var_neq_sym xR yR Hneq)) v)
+     as Henc'. rewrite Hcall2 in Henc'. cbn in *. rewrite Henc'. auto.
+  - specialize (call_mrec_encodes t1 t2 _ _ xt xR v) as Henc.
+    rewrite <- Henc. rewrite Hcall1. auto.
+Qed.
