theories/AlmostStlc/MapEFacts.v
@@ -1,0 +1,156 @@
+From Coq Require Import
+     Program
+     Setoid
+     Morphisms
+     Relations
+     Logic.FunctionalExtensionality
+.
+
+From Paco Require Import paco.
+
+From ITree Require Import
+     Basics.Basics
+     Basics.Monad
+     Basics.Tacs
+     Basics.HeterogeneousRelations
+     Eq.Paco2.
+
+From EnTree Require Import
+     Basics.HeterogeneousRelations
+     Core.EnTreeDefinition
+     Core.SubEvent
+     Eq.Eqit
+.
+
+Require Import ExtLib.Structures.Functor.
+Require Import ExtLib.Structures.Applicative.
+Require Import ExtLib.Structures.Monad.
+Require Import Program.Tactics.
+
+Require Import ITree.Basics.Basics.
+
+Require Export TypedVar MrecMonad.
+
+From Equations Require Import Equations Signature.
+
+(* possibly should further generalize to having input and output rel *)
+Definition handler_eq {D1 D2 : Type} `{EncodedType D1} `{EncodedType D2} (Rd : D1 -> D1 -> Prop) (h1 h2 : handler D1 D2) : Prop :=
+  forall (d1 d1' : D1), Rd d1 d1' -> 
+                   (projT1 (h1 d1)) = (projT1 (h2 d1')) /\
+                     projT2 (h1 d1) ~= (@id (encodes d1)) /\
+                     projT2 (h2 d1') ~= (@id (encodes d1')) /\ 
+                     encodes d1 = encodes ((projT1 (h1 d1))) /\ 
+                     encodes d1' = encodes (projT1 (h2 d1'))
+.
+
+Class valid_handler {D1 D2 : Type} `{EncodedType D1} `{EncodedType D2} (h : handler D1 D2) : Prop :=
+   valid : forall d1, encodes d1 = encodes (projT1 (h d1)) /\ projT2 (h d1) ~= (@id (encodes d1)).
+
+Lemma valid_handler_self_eq {D1 D2 : Type} `{EncodedType D1} `{EncodedType D2} (h : handler D1 D2) : 
+  valid_handler h <-> handler_eq eq h h.
+Proof.
+  unfold valid_handler, handler_eq. split; intros; subst; eauto.
+  - specialize (H1 d1'). destruct H1. repeat split; auto.
+  - specialize (H1 d1 d1 eq_refl). tauto.
+Qed.
+
+
+Section mapE_match.
+Context (D1 D2 : Type) `{EncodedType D1} `{EncodedType D2}.
+Context (h : handler D1 D2).
+
+Lemma mapE_ret R (r : R) : mapE h (ret r) ≅ ret r.
+Proof.
+  pstep. red. constructor. auto.
+Qed.
+
+Lemma mapE_tau R (t : entree D1 R) : mapE h (Tau t) ≅ Tau (mapE h t).
+Proof.
+  pstep. red. cbn. constructor. left. apply Reflexive_eqit. auto.
+Qed.
+
+Lemma mapE_vis R (d : D1) (k : encodes d -> entree D1 R) : 
+  mapE h (Vis d k) ≅ 
+       let '(d' && f) := h d in
+       Vis d' (fun x => mapE h (k (f x))).
+Proof.
+  pstep. red.
+  unfold mapE at 1. cbn. 
+  destruct (h d) eqn : Hhd. cbn.
+  unfold observe, _observe. cbn. rewrite Hhd. constructor. left.
+  apply Reflexive_eqit. auto.
+Qed.
+End mapE_match.
+
+
+Section mapE_proper.
+Context (D1 D2 : Type) `{EncodedType D1} `{EncodedType D2}.
+(* maybe can further generalize *)
+Context (h1 h2 : handler D1 D2) (Hh : handler_eq eq h1 h2).
+
+Lemma mapE_proper b1 b2 (R : Type) (t1 t2 : entree D1 R) : eqit eq b1 b2 t1 t2 -> eqit eq b1 b2 (mapE h1 t1) (mapE h2 t2).
+Proof.
+  ginit.
+  revert t1 t2. gcofix CIH. intros t1 t2 Ht12.
+  punfold Ht12. red in Ht12. unfold mapE.
+  hinduction Ht12 before r; intros; subst; try inv CHECK.
+  - gstep. red. cbn. constructor. auto.
+  - gstep. red. cbn. constructor. gfinal. pclearbot. eauto.
+  - setoid_rewrite mapE_vis. specialize (Hh e e eq_refl).
+    destruct (h1 e). destruct (h2 e). cbn in Hh. decompose record Hh. subst.
+    gstep. constructor. pclearbot. intros.
+    remember (encodes e) as B. remember (encodes x0) as A. clear HeqB HeqA. subst.
+    apply JMeq_eq in H2, H3. subst. gfinal. left. eapply CIH. apply REL.
+  - setoid_rewrite mapE_tau. rewrite tau_euttge. eapply IHHt12. eauto.
+  - setoid_rewrite mapE_tau. rewrite tau_euttge. eapply IHHt12. eauto.
+Qed.
+
+End mapE_proper.
+
+
+#[global] Instance mapE_proper_inst {b1 b2} {D1 D2 : Type} `{EncodedType D1} `{EncodedType D2} {R}: 
+  Proper (@handler_eq D1 D2 _ _ eq ==> eqit (@eq R) b1 b2 ==> eqit eq b1 b2) mapE.
+Proof.
+  repeat intro. apply mapE_proper; auto.
+Qed.
+Arguments valid_handler {_ _ _ _}.
+Section test.
+Context (D1 D2 : Type) `{enc1 : EncodedType D1} `{enc2 : EncodedType D2}.
+Context (h : handler D1 D2) (H : valid_handler h).
+
+End test.
+
+#[global] Instance mapE_proper_inst_const_h {b1 b2} {D1 D2 : Type} `{enc1 : EncodedType D1} `{enc2 : EncodedType D2} {R} 
+ (h : handler D1 D2) `{@valid_handler D1 D2 enc1 enc2 h} :
+  Proper (eqit (@eq R) b1 b2 ==> eqit eq b1 b2) (mapE h).
+Proof. 
+  apply mapE_proper_inst.
+  apply valid_handler_self_eq. auto.
+Qed.
+  
+#[global] Instance mapE_proper_inst_const_h_eutt {D1 D2 : Type} `{enc1 : EncodedType D1} `{enc2 : EncodedType D2} {R} h
+  `{@valid_handler D1 D2 enc1 enc2 h}: 
+  Proper (eutt eq ==> eutt (@eq R)) (mapE h).
+Proof. apply mapE_proper_inst_const_h. auto. Qed.
+
+Section mapE_bind.
+Context (D1 D2 : Type) `{EncodedType D1} `{EncodedType D2}.
+(* maybe can further generalize *)
+(* this validiity condition*)
+Context (h : handler D1 D2) (Hvalid : valid_handler h).
+
+Lemma mapE_bind R S (m : entree D1 R) (k : R -> entree D1 S) : 
+  mapE h (bind m k) ≅ bind (mapE h m) (fun r => mapE h (k r)).
+Proof.
+  revert m. ginit. gcofix CIH. intros.
+  destruct (observe m) eqn : Heq; symmetry in Heq; apply simpobs in Heq.
+  - setoid_rewrite <- Heq. setoid_rewrite mapE_ret. setoid_rewrite bind_ret_l.
+    apply Reflexive_eqit_gen. auto.
+  - setoid_rewrite <- Heq. setoid_rewrite mapE_tau. setoid_rewrite bind_tau.
+    gstep. constructor. gfinal. left. eapply CIH.
+  - setoid_rewrite <- Heq. setoid_rewrite mapE_vis. specialize (Hvalid e).
+    destruct (h e). cbn in Hvalid. setoid_rewrite bind_vis. gstep. constructor.
+    gfinal. left. eapply CIH.
+Qed.
+
+End mapE_bind.
