theories/AlmostStlc/Tactics.v
@@ -1,0 +1,3 @@
+
+
+(* Ltac force f := Transparent f; simpl f; Opaque f. *)
