theories/Eq/Eqit.v
@@ -93,6 +93,19 @@ Ltac unfold_eqit :=
   (try match goal with [|- eqit_ _ _ _ _ _ _ _ ] => red end);
   (repeat match goal with [H: eqit_ _ _ _ _ _ _ _ |- _ ] => red in H end).
 
+Lemma eqit_Ret {E R1 R2} `{EncodedType E} b1 b2 (RR : R1 -> R2 -> Prop) r1 r2 : 
+  RR r1 r2 -> eqit RR b1 b2 (Ret r1) (Ret r2).
+Proof.
+  intros. pstep. constructor. auto.
+Qed.
+
+Lemma eqit_Vis {E R1 R2} `{EncodedType E} b1 b2 (RR : R1 -> R2 -> Prop) (e : E) k1 k2 :
+  (forall a, eqit RR b1 b2 (k1 a) (k2 a)) -> eqit RR b1 b2 (Vis e k1) (Vis e k2).
+Proof.
+  intros. pstep. constructor.
+  intros. left. apply H0.
+Qed.
+
 Lemma eqit_Vis_inv {E R1 R2} `{EncodedType E} b1 b2 (RR : R1 -> R2 -> Prop) (e : E) k1 k2 :
   eqit RR b1 b2 (Vis e k1) (Vis e k2) -> forall a, eqit RR b1 b2 (k1 a) (k2 a).
 Proof.
