theories/Eq/Rutt.v
@@ -1,0 +1,19 @@
+From Coq Require Import
+     Program
+     Setoid
+     Morphisms
+     Relations.
+
+From Paco Require Import paco.
+
+From ITree Require Import
+     Basics.Basics
+     Basics.Tacs
+     Basics.HeterogeneousRelations
+     Eq.Paco2.
+
+From EnTree Require Import
+     Basics.HeterogeneousRelations
+     Core.EnTreeDefinition.
+
+Local Open Scope entree_scope.
